backend/Cminor.v
@@ -445,6 +445,7 @@ Inductive step: state -> trace -> state -> Prop :=
   | step_skip_call: forall f k sp e m m',
       is_call_cont k ->
       Mem.free m sp 0 f.(fn_stackspace) = Some m' ->
+      Mem.stack (Mem.support m') <> nil ->
       step (State f Sskip k (Vptr sp Ptrofs.zero) e m)
         E0 (Returnstate Vundef k m')
 
@@ -476,6 +477,7 @@ Inductive step: state -> trace -> state -> Prop :=
       Genv.find_funct ge vf = Some fd ->
       funsig fd = sig ->
       Mem.free m sp 0 f.(fn_stackspace) = Some m' ->
+      Mem.stack (Mem.support m') <> nil ->
       step (State f (Stailcall sig a bl) k (Vptr sp Ptrofs.zero) e m)
         E0 (Callstate fd vargs (call_cont k) m' (fn_stack_requirements id))
 
@@ -522,11 +524,13 @@ Inductive step: state -> trace -> state -> Prop :=
 
   | step_return_0: forall f k sp e m m',
       Mem.free m sp 0 f.(fn_stackspace) = Some m' ->
+      Mem.stack(Mem.support m') <> nil ->
       step (State f (Sreturn None) k (Vptr sp Ptrofs.zero) e m)
         E0 (Returnstate Vundef (call_cont k) m')
   | step_return_1: forall f a k sp e m v m',
       eval_expr (Vptr sp Ptrofs.zero) e m a v ->
       Mem.free m sp 0 f.(fn_stackspace) = Some m' ->
+      Mem.stack(Mem.support m') <> nil ->
       step (State f (Sreturn (Some a)) k (Vptr sp Ptrofs.zero) e m)
         E0 (Returnstate v (call_cont k) m')
 
@@ -656,8 +660,8 @@ Proof.
   + assert (id = id0). eapply function_id_determ; eauto.
     subst vf0 vargs0 id0. rewrite H4 in H18. inv H18. auto.
   + assert (id = id0). eapply function_id_determ; eauto.
-    subst vf0 vargs0 id0. rewrite H4 in H18. inv H18.
-    rewrite H6 in H20. inv H20. auto.
+    subst vf0 vargs0 id0. rewrite H4 in H19. inv H19.
+    rewrite H6 in H21. inv H21. auto.
   + subst vargs0. exploit external_call_determ. eexact H2. eexact H14.
     intros (A & B). split; intros; auto.
     apply B in H; destruct H; congruence.
