backend/CminorSel.v
@@ -345,6 +345,7 @@ Inductive step: state -> trace -> state -> Prop :=
   | step_skip_call: forall f k sp e m m',
       is_call_cont k ->
       Mem.free m sp 0 f.(fn_stackspace) = Some m' ->
+      Mem.stack (Mem.support m') <> nil ->
       step (State f Sskip k (Vptr sp Ptrofs.zero) e m)
         E0 (Returnstate Vundef k m')
 
@@ -377,6 +378,7 @@ Inductive step: state -> trace -> state -> Prop :=
       Genv.find_funct ge vf = Some fd ->
       funsig fd = sig ->
       Mem.free m sp 0 f.(fn_stackspace) = Some m' ->
+      Mem.stack (Mem.support m') <> nil ->
       step (State f (Stailcall sig a bl) k (Vptr sp Ptrofs.zero) e m)
         E0 (Callstate fd vargs (call_cont k) m' (fn_stack_requirements id))
 
@@ -421,11 +423,13 @@ Inductive step: state -> trace -> state -> Prop :=
 
   | step_return_0: forall f k sp e m m',
       Mem.free m sp 0 f.(fn_stackspace) = Some m' ->
+      Mem.stack (Mem.support m') <> nil ->
       step (State f (Sreturn None) k (Vptr sp Ptrofs.zero) e m)
         E0 (Returnstate Vundef (call_cont k) m')
   | step_return_1: forall f a k sp e m v m',
       eval_expr (Vptr sp Ptrofs.zero) e m nil a v ->
       Mem.free m sp 0 f.(fn_stackspace) = Some m' ->
+      Mem.stack (Mem.support m') <> nil ->
       step (State f (Sreturn (Some a)) k (Vptr sp Ptrofs.zero) e m)
         E0 (Returnstate v (call_cont k) m')
 
